---
title: "STAT_5361_Hw8_(1)"
author: "Yicheng Guo"
date: "2020/10/31"
output: pdf_document
---

```{r setup, include=FALSE}
knitr::opts_chunk$set(echo = TRUE)
```

By Ito's formula, let $H(t) = \int_0^t -adt = -at$,
$$
\begin{aligned}
  & d[e^{-H(t)}r(t)] = e^{-H(t)}g(t)dt + e^{-H(t)}\sigma(t) dW(t), \\
  & d[e^{at}r(t)] = e^{at}*ab*dt + e^{at}\sigma dW(t), \\
  & r(t+\triangle) = e^{-a\triangle}r(t) + ab\int_t^{\triangle + t} (e^{as - at})ds +
  \sigma \int_t^{\triangle + t} (e^{as - at})dW(s) \\
  & = e^{-a\triangle}r(t) + b(1 - e^{-a\triangle}) + 
  \sigma \int_0^{\triangle} (e^{as}) dW(s+t)
\end{aligned}
$$

Finally, we need to prove that

$$
\begin{aligned}
& \sigma \int_0^{\triangle} (e^{as}) dW(s+t) = \sigma \int_0^{\triangle} (e^{as}) dW(s) = \frac{\sigma}{\sqrt{2a}}
\sqrt{1 - e^{-2a\triangle}} Z
\end{aligned}
$$

By Ito's isometry, 

$$
  E[(\int_0^\triangle e^{as} dW(s))^2] = \int_0^\triangle (e^{as})^2 ds = \frac{1 - e^{-2a\triangle}}{2a}
$$

Therefore

$$
  (\int_0^\triangle e^{as} dW(s))^2 \sim \frac{1 - e^{-2a\triangle}}{2a} \chi^2_{(1)},
$$
$$
    \int_0^\triangle e^{as} dW(s) \sim \sqrt{\frac{1 - e^{-2a\triangle}}{2a}} Z.
$$

which complete the proof.